lawyer/nonblocking/tokens/pr_wfree_tokens.v
@@ -2,7 +2,7 @@ From iris.proofmode Require Import tactics.
 From trillium.traces Require Import inftraces trace_lookup exec_traces trace_len trace_utils. 
 From fairness Require Import fairness locales_helpers.
 From lawyer.obligations Require Import obligations_resources obligations_logic env_helpers obligations_adequacy obligations_model obligations_em obligations_am obls_termination obligations_wf.
-From lawyer.nonblocking Require Import trace_context om_wfree_inst wptp_gen pwp wfree_traces calls.
+From lawyer.nonblocking Require Import trace_context om_wfree_inst wptp_gen pwp wfree_traces calls pr_wfree_lib.
 From lawyer.nonblocking.tokens Require Import pwp_ext om_wfree_inst_tokens.
 From trillium.program_logic Require Import execution_model weakestpre adequacy_utils adequacy_cond simulation_adequacy_em_cond. 
 From lawyer Require Import action_model sub_action_em.
@@ -33,17 +33,6 @@ Section WaitFreePR.
   
   Open Scope WFR_scope. 
 
-  Local Definition OHE {Σ} {Hinv : @IEMGS _ _ HeapLangEM EM Σ}:
-    OM_HL_Env OP_HL_WF EM Σ.
-  esplit. 
-  - apply AMU_lift_top.
-  - intros.
-    iIntros. iApply AMU_lift_top; [(try rewrite nclose_nroot); done| ].
-    iFrame.
-  Unshelve.
-  exact {| heap_iemgs := Hinv |}.
-  Defined.
-
   Lemma get_call_wp {Σ} {Hinv : @IEMGS _ _ HeapLangEM EM Σ} {UT: UnitToken Σ}
     (a: val) π:
     let _: ObligationsGS Σ := @iem_fairnessGS _ _ _ _ _ Hinv in
@@ -60,15 +49,12 @@ Section WaitFreePR.
     apply phase_le_init.
   Qed.
 
-  Definition no_extra_obls (_: cfg heap_lang) (δ: mstate M) :=
-    forall τ', default ∅ (ps_obls δ !! τ') ≠ ∅ -> τ' = τi.
-
-  Definition obls_sim_rel_wfree extr omtr :=
-    obls_sim_rel extr omtr /\ no_extra_obls (trace_last extr) (trace_last omtr).
+  (* Definition obls_sim_rel_wfree extr omtr := *)
+  (*   obls_sim_rel extr omtr /\ no_extra_obls (trace_last extr) (trace_last omtr). *)
 
   Definition wfree_trace_inv `{Hinv : @IEMGS _ _ HeapLangEM EM Σ}
     (extr: execution_trace heap_lang) (omtr: auxiliary_trace M): iProp Σ :=
-    ⌜ no_extra_obls (trace_last extr) (trace_last omtr) /\
+    ⌜ no_extra_obls ic (trace_last extr) (trace_last omtr) /\
       from_option (fun e => to_val e = None) True (from_locale (trace_last extr).1 τi) ⌝ ∗
     (let _: heap1GS Σ := iem_phys HeapLangEM EM in wfst_mod_inv _ WFST). 
   
@@ -177,156 +163,11 @@ Section WaitFreePR.
     Unshelve. all: by apply trace_singleton. 
   Qed. 
 
-  Definition extra_fuel `{!ObligationsGS Σ} (etr: execution_trace heap_lang) :=
-    let len := trace_length etr in
-    if len <=? ii then (cp_mul π0 d0 (S ii - len) ∗ cp_mul π0 d0 F)%I else ⌜ True ⌝%I.
-
-  Definition cur_phases `{!ObligationsGS Σ} (etr: execution_trace heap_lang): iProp Σ :=
-    let c := trace_last etr in
-    ([∗ set] τ ∈ locales_of_cfg c ∖ {[ τi ]}, ∃ π, th_phase_eq τ π) ∗
-    let ph_res := let q := if (trace_length etr <=? ii) then 1%Qp else (/2)%Qp in
-                  (∃ π, th_phase_frag τi π q)%I in
-    ⌜ τi ∈ locales_of_cfg c ⌝ → ph_res.
-
-  Definition obls_τi `{!ObligationsGS Σ}: iProp Σ :=
-    ∃ s, obls τi {[ s ]} ∗ sgn s l0 (Some false) ∗ ep s π0 d0. 
-
-  Definition obls_τi' `{!ObligationsGS Σ} (c: cfg heap_lang): iProp Σ :=
-    if decide (τi ∈ locales_of_cfg c) then obls_τi else cp π0 d1.
-
-  Definition cur_obls_sigs `{!ObligationsGS Σ} (etr: execution_trace heap_lang): iProp Σ :=
-    let c := trace_last etr in
-    ([∗ set] τ ∈ locales_of_cfg c ∖ {[ τi ]}, obls τ ∅) ∗
-    obls_τi' c. 
-
   Definition pr_pr_wfree {Σ} {PWT: PrWfreeTok Σ}
     (s: stuckness) (etr: execution_trace heap_lang) (Φs: list (val → iProp Σ)): iProp Σ :=
     let oGS: ObligationsGS Σ := @iem_fairnessGS _ _ _ _ _ (@pwt_Hinv _ PWT) in
-    wptp_wfree s etr Φs ∗ extra_fuel etr ∗ cur_phases etr ∗
-    cur_obls_sigs etr ∗ cti_cond etr. 
-
-  (* TODO: remove? *)
-  Lemma cur_phases_take `{!ObligationsGS Σ} etr τ
-    (IN: τ ∈ locales_of_cfg (trace_last etr)):
-    let ph π := th_phase_frag τ π (/2)%Qp in
-    cur_phases etr ⊣⊢ ∃ π, ph π ∗ (ph π -∗ cur_phases etr).
-  Proof using.
-    simpl. rewrite /cur_phases.
-    destruct (decide (τ = τi)) as [-> | NEQ]. 
-    - iSplit.
-      2: { iIntros "(%π & PH & CLOS)".
-           by iApply "CLOS". }
-      iIntros "[PHS' PH]". iDestruct ("PH" with "[//]") as (π) "PH".
-      erewrite th_phase_frag_combine' with (p := (/ 2)%Qp).
-      2: { by destruct Nat.leb. }
-      iDestruct "PH" as "[PH PH']".
-      iExists π. iFrame.
-      iIntros "PH _".
-      iExists _. iApply th_phase_frag_combine'; [| by iFrame].
-      by destruct Nat.leb.
-    - iSplit.
-      2: { iIntros "(%π & PH & CLOS)".
-           by iApply "CLOS". }
-      iIntros "[PHS' PH]". iFrame "PH".
-      iDestruct (big_sepS_elem_of_acc with "[$]") as "[PH PHS]".
-      { apply elem_of_difference. split; eauto. set_solver. }
-      iDestruct "PH" as "(%π & PH)".
-      rewrite {1}/th_phase_eq. rewrite -Qp.inv_half_half. 
-      iDestruct (th_phase_frag_combine with "PH") as "[PH1 PH2]".
-      iExists _. iFrame.
-      iIntros "PH". iApply "PHS".
-      iExists _. iEval (rewrite /th_phase_eq).
-      rewrite -Qp.inv_half_half. iApply th_phase_frag_combine. iFrame.
-  Qed.
-
-  (* TODO: refactor *)
-  Lemma same_phase_no_fork {Σ} {Hinv : @IEMGS _ _ HeapLangEM EM Σ}
-    etr mtr
-    (e : expr)
-    (σ σ' : state)
-    (efs t1 t2 : list expr)
-    (FIN : trace_last etr = (t1 ++ e :: t2, σ))
-    (ec : expr)
-    (π : Phase)
-    (PH : ps_phases (trace_last mtr) !! τi = Some π)
-    (CORR : obls_cfg_corr (trace_last etr) (trace_last mtr))
-    (x : expr)
-    (H2 : prim_step ec σ x σ' efs)
-    (δ' : AM2M ObligationsAM)
-    (ℓ : mlabel (AM2M ObligationsAM)):
-   ⊢ @th_phase_frag _ _ _ WF_SB OP Σ
-           (@iem_fairnessGS heap_lang _ HeapLangEM EM Σ Hinv)
-           τi π (/ 2) -∗
-  ⌜@obls_ves_wrapper _ _ _ WF_SB
-             OP Nat.inhabited (@trace_last (cfg heap_lang) (option nat) etr)
-             (@Some nat τi)
-             (t1 ++ @fill _ Ki x :: t2 ++ efs, σ')
-             (trace_last mtr)
-             ℓ δ'⌝ ∗
-          @gen_heap_interp loc loc_eq_decision loc_countable (option val) Σ
-            (@heap_gen_heapGS Σ (@iem_phys heap_lang _ HeapLangEM EM Σ Hinv))
-            (heap σ') ∗
-          @obls_asem_mti _ _ _ WF_SB OP
-            Nat.inhabited Σ
-            (@iem_fairnessGS heap_lang _ HeapLangEM EM Σ Hinv)
-            (etr :tr[ @Some nat τi]: (t1 ++ @fill _ Ki x :: t2 ++ efs, σ'))
-            (mtr :tr[ ℓ ]: δ') -∗
-  ⌜efs = [] /\ locales_of_cfg (trace_last etr) = locales_of_cfg (t1 ++ @fill _ Ki x :: t2 ++ efs, σ')⌝.
-  Proof using.
-    clear m WFST F.
-    iIntros "PH HSI".
-    iAssert (⌜ ps_phases δ'  !! τi = Some π ⌝)%I as "%PH'".
-    { iApply (th_phase_msi_frag with "[-PH] [$]").
-      by iDestruct "HSI" as "(?&?&(?&?&?))". }
-    iDestruct "HSI" as "(%EVOL&_&CORR')".
-    rewrite /obls_asem_mti. simpl. 
-    red in EVOL. destruct ℓ as [? [|]].
-    2: { tauto. } 
-    destruct EVOL as [MSTEP ->]. simpl in MSTEP.
-    red in MSTEP. destruct MSTEP as (_ & MSTEP & [=<-] & CORR').
-    simpl in MSTEP.
-    
-    (* TODO: make a lemma *)
-    assert (ps_phases (trace_last mtr) = ps_phases δ') as PH_EQ.
-    { destruct MSTEP as (δ2 & PSTEP & OFORK).
-      destruct PSTEP as (? & ? & δ1 & STEPS & BURN).
-      assert (ps_phases (trace_last mtr) = ps_phases δ2) as EQ2. 
-      { rewrite (lse_rep_phases_eq_helper _ _ _ STEPS).
-        destruct BURN as (?&?&BURN).
-        eapply lse_rep_phases_eq_helper.
-        apply nsteps_once. red. left.
-        eexists. red. eauto. }
-      inversion OFORK.
-      2: { by subst. }
-      subst y. red in H0. destruct H0 as (?&?&FORK).
-      inversion FORK. subst.
-      subst ps'. rewrite phases_update_phases in PH'.
-      subst new_phases0.
-      rewrite lookup_insert_ne in PH'.
-      2: { intros ->. destruct FRESH'. by eapply elem_of_dom. }
-      rewrite lookup_insert in PH'. inversion PH'.
-      rewrite -EQ2 PH in LOC_PHASE. inversion LOC_PHASE. subst π0.
-      pose proof (phase_lt_fork π 0) as NEQ. red in NEQ.
-      apply strict_ne in NEQ. done. }
-    
-    red in CORR'. destruct CORR' as (CORR' & DPO').
-
-    rewrite (proj1 CORR) (CORR'). 
-
-    red in DPO'. apply (@f_equal _ _ dom) in PH_EQ. 
-    rewrite DPO' in PH_EQ.
-    red in CORR'. rewrite -PH_EQ in CORR'.
-    red in CORR. rewrite (proj2 CORR) -(proj1 CORR) in CORR'.
-    rewrite FIN in CORR'. simpl in CORR.
-    rewrite !locales_of_cfg_simpl in CORR'.
-    repeat (rewrite !length_app /= in CORR').
-
-     iPureIntro. split.
-     2: { set_solver. }
-    
-    destruct efs; [done| ].
-    simpl in CORR'. apply set_seq_uniq2 in CORR'. lia.
-  Qed.
+    wptp_wfree s etr Φs ∗ extra_fuel ic F etr ∗ cur_phases ic etr ∗
+    cur_obls_sigs ic etr ∗ cti_cond etr. 
 
   Lemma reestablish_wfree_inv {Σ} {Hinv : @IEMGS _ _ HeapLangEM EM Σ}
     etr mtr
@@ -334,7 +175,7 @@ Section WaitFreePR.
     :
     let _: ObligationsGS Σ := @iem_fairnessGS _ _ _ _ _ Hinv in
     (let _: heap1GS Σ := iem_phys HeapLangEM EM in wfst_mod_inv _ WFST) -∗
-    cur_obls_sigs etr -∗ state_interp etr mtr -∗
+    cur_obls_sigs ic etr -∗ state_interp etr mtr -∗
     wfree_trace_inv etr mtr.
   Proof using.
     simpl. iIntros "#INV OB TI".
@@ -363,361 +204,6 @@ Section WaitFreePR.
       2: { simpl. rewrite -Nat.sub_succ_l; [lia| ].
            destruct etr; simpl; lia. }
       done. 
-  Qed.
-
-  Lemma split_trace_fuel {Σ} {Hinv : @IEMGS _ _ HeapLangEM EM Σ}
-    etr c' τ
-    (BEFORE: trace_length etr <= ii):
-    let _: ObligationsGS Σ := @iem_fairnessGS _ _ _ _ _ Hinv in
-    let fuel_pre := cp_mul π0 d0 F in
-    ⊢ extra_fuel etr -∗ cp π0 d0 ∗ fuel_pre ∗
-      ((⌜ trace_length etr < ii ⌝ → fuel_pre) -∗ extra_fuel (etr :tr[ Some τ]: c')).
-  Proof using.
-    simpl. iIntros "CPS". 
-    rewrite /extra_fuel.
-    rewrite leb_correct; [| done]. 
-    rewrite Nat.sub_succ_l; [| done]. rewrite cp_mul_take.
-    iDestruct "CPS" as "((CPS & CP) & CPP)". iFrame.
-    iIntros "CPP".
-    destruct leb eqn:LEN; [| done]. iFrame.
-    iApply "CPP". iPureIntro. 
-    apply leb_complete in LEN. simpl in LEN. lia.
-  Qed.
-
-  Lemma reestablish_fuel {Σ} {Hinv : @IEMGS _ _ HeapLangEM EM Σ}
-    etr c' τ:
-    let _: ObligationsGS Σ := @iem_fairnessGS _ _ _ _ _ Hinv in
-    ⊢ extra_fuel etr -∗ extra_fuel (etr :tr[ Some τ]: c').
-  Proof using.
-    simpl. iIntros "CPS". 
-    rewrite /extra_fuel.
-    destruct (trace_length (_ :tr[ _ ]: _) <=? _) eqn:LE; [| done].
-    rewrite leb_correct.
-    2: { apply leb_complete in LE. simpl in *. lia. }
-    simpl. iDestruct "CPS" as "(? & $)".
-    iApply (cp_mul_weaken with "[$]"); [done| lia].
-  Qed.
-
-  Lemma reestablish_phases {Σ} {Hinv : @IEMGS _ _ HeapLangEM EM Σ}
-    etr τ c'
-    (EQ_CFG: locales_of_cfg (trace_last etr) = locales_of_cfg c')
-    (AFTER: ii < trace_length etr)
-    :
-    let _: ObligationsGS Σ := @iem_fairnessGS _ _ _ _ _ Hinv in
-    cur_phases etr -∗ cur_phases (etr :tr[ Some τ ]: c').
-  Proof using.
-    clear m WFST F.
-    simpl. iIntros "PHS".
-    rewrite /cur_phases.
-    rewrite -EQ_CFG.    
-    rewrite leb_correct_conv; [| done].
-    rewrite leb_correct_conv; [done| ].
-    simpl.
-    remember (trace_length etr) as X. rewrite -HeqX. lia.
-  Qed.
-
-  Lemma reestablish_obls_sigs {Σ} {Hinv : @IEMGS _ _ HeapLangEM EM Σ}
-    etr t1 t2 x σ'
-    (EQ_CFG: locales_of_cfg (trace_last etr) = locales_of_cfg (t1 ++ fill Ki x :: t2, σ')):
-    let _: ObligationsGS Σ := @iem_fairnessGS _ _ _ _ _ Hinv in
-    cur_obls_sigs etr -∗ cur_obls_sigs (etr :tr[ Some τi ]: (t1 ++ fill Ki x :: t2, σ')).
-  Proof using.
-    simpl. iIntros "(OBS & OBτi)". 
-    rewrite /cur_obls_sigs. simpl.
-    rewrite /obls_τi'. 
-    rewrite -EQ_CFG. iFrame. 
-  Qed.
-
-  From lawyer Require Import program_logic.  
-
-  Lemma MU_burn_cp_nofork {Σ} {Hinv : @IEMGS _ _ HeapLangEM EM Σ} τ π d q P:
-    let _: ObligationsGS Σ := @iem_fairnessGS _ _ _ _ _ Hinv in
-    ⊢ BOU ∅ WF_SB (cp π d ∗ th_phase_frag τ π q ∗ P) -∗ 
-      let hGS: @heapGS Σ M EM := {| heap_iemgs := Hinv |} in
-      @MU _ EM Σ hGS ⊤ τ (th_phase_frag τ π q ∗ P).
-  Proof using.
-    simpl. iIntros "BOU".
-    iApply AMU_lift_top; [(try rewrite nclose_nroot); done| ].
-    iApply BOU_AMU. iApply (BOU_weaken with "[] [$]"); try done.
-    iIntros "(CP & PH & P)".
-    iSplitL "P".
-    { by iIntros "$". }
-    iFrame.
-  Qed.
-
-  Lemma MU_burn_cp_fork {Σ} {Hinv : @IEMGS _ _ HeapLangEM EM Σ} τ π0 d τ' Q:
-    let _: ObligationsGS Σ := @iem_fairnessGS _ _ _ _ _ Hinv in
-    ⊢ BOU ∅ WF_SB (∃ R1 R2, cp π0 d ∗ th_phase_eq τ π0 ∗ obls τ (R1 ∪ R2) ∗ Q R1 R2 ∗ ⌜ R1 ## R2 ⌝) -∗
-      let hGS: @heapGS Σ M EM := {| heap_iemgs := Hinv |} in
-      @MU__f _ EM Σ hGS ⊤ τ τ'
-        (∃ π π' R1 R2, th_phase_eq τ π ∗ th_phase_eq τ' π' ∗ obls τ R1 ∗ obls τ' R2 ∗ Q R1 R2 ∗ ⌜ R1 ## R2 ⌝).
-  Proof using.
-    simpl. iIntros "BOU".
-    iApply AMU_lift_top; [(try rewrite nclose_nroot); done| ].
-    iApply (BOU_AMU__f'_strong _ _ _ _ Q). iApply (BOU_weaken with "[] [$]"); try done. 
-    iIntros "(%R1 & %R2 & CP & PH & OB & Q &?)".
-    iFrame. 
-    iIntros "(%&%&%&%&?&?&?&?&?&?)".
-    iFrame. 
-  Qed.
-
-  Lemma MU_burn_cp {Σ} {Hinv : @IEMGS _ _ HeapLangEM EM Σ} τ π0 d oτ' Q:
-    let _: ObligationsGS Σ := @iem_fairnessGS _ _ _ _ _ Hinv in
-    ⊢ BOU ∅ WF_SB (∃ R1 R2, cp π0 d ∗ th_phase_eq τ π0 ∗ obls τ (R1 ∪ R2) ∗ Q R1 R2 ∗ ⌜ R1 ## R2 ⌝) -∗
-      let hGS: @heapGS Σ M EM := {| heap_iemgs := Hinv |} in
-      @MU_impl _ EM Σ hGS oτ' ⊤ τ
-        (∃ π R1 R2, th_phase_eq τ π ∗ Q R1 R2 ∗ ⌜ R1 ## R2 ⌝ ∗
-         from_option (fun τ' => ∃ π', th_phase_eq τ' π' ∗ obls τ R1 ∗ obls τ' R2) (obls τ (R1 ∪ R2)) oτ').
-  Proof using.
-    simpl. iIntros "BOU".
-    destruct oτ'.
-    - iPoseProof (MU_burn_cp_fork with "[$]") as "foo".
-      iApply (MU__f_wand with "[] [$]"). simpl.
-      iIntros "(%&%&%&%&?&?&?&?&?)". by iFrame.
-    - simpl.
-      iApply (MU_wand with "[-BOU]").
-      2: { iApply MU_burn_cp_nofork. iMod "BOU".
-           repeat setoid_rewrite <- bi.sep_exist_l. 
-           iModIntro. iFrame. }
-      iIntros "[$ X]". by iDestruct "X" as "(%&%&$&?)". 
-  Qed.
-
-  Lemma cur_obls_sigs_τi_step `{!ObligationsGS Σ} etr c'
-    (STEP: locale_step (trace_last etr) (Some τi) c'):
-    cur_obls_sigs etr -∗ obls_τi ∗
-      let oτ' := step_fork (trace_last etr) c' in
-      (obls_τi -∗ from_option (fun τ' => obls τ' ∅) ⌜ True ⌝ oτ' -∗ cur_obls_sigs (etr :tr[ Some τi ]: c')).
-  Proof using.
-    simpl. iIntros "(OBLS & OB)".
-    rewrite /cur_obls_sigs /obls_τi'. simpl.
-    rewrite decide_True.
-    2: { eapply locales_of_cfg_step; eauto. }
-    iFrame. iIntros "OB OB'". 
-    rewrite decide_True.
-    2: { eapply locale_step_sub; eauto. eapply locales_of_cfg_step; eauto. }
-    iFrame.
-    pose proof STEP as ->%locale_step_step_fork_exact. 
-    rewrite difference_union_distr_l_L big_sepS_union.
-    2: { destruct step_fork eqn:SF; [| set_solver].
-         simpl. apply elem_of_disjoint.
-         intros ? [??]%elem_of_difference [->%elem_of_singleton ?]%elem_of_difference.
-         apply step_fork_difference in SF. set_solver. }
-    iFrame. destruct step_fork eqn:SF; simpl. 
-    2: { rewrite subseteq_empty_difference_L; set_solver. }
-    rewrite difference_disjoint_L.
-    2: { apply step_fork_difference in SF.
-         apply locales_of_cfg_step in STEP.
-         set_solver. }
-    by rewrite big_sepS_singleton.
-  Qed.
-
-  Lemma cur_phases_τi_step `{!ObligationsGS Σ} etr c'
-    (STEP: locale_step (trace_last etr) (Some τi) c'):
-    cur_phases etr -∗
-    let oτ' := step_fork (trace_last etr) c' in
-    let ph ex := ∃ π, th_phase_frag τi π (if (trace_length ex <=? ii) then 1%Qp else (/2)%Qp) in
-    let etr' := etr :tr[ Some τi ]: c' in
-    ph etr ∗ (ph etr' -∗ from_option (fun τ' => ∃ π', th_phase_eq τ' π') ⌜ True ⌝ oτ' -∗ cur_phases etr').
-  Proof using.
-    #[local] Arguments Nat.leb _ _ : simpl nomatch.
-    rewrite /cur_phases. simpl. iIntros "(PHS & PH)".
-    iSpecialize ("PH" with "[]").
-    { iPureIntro. eapply locales_of_cfg_step; eauto. }
-    iFrame.
-    iIntros "PH PH'".
-    pose proof STEP as ->%locale_step_step_fork_exact. 
-    rewrite difference_union_distr_l_L big_sepS_union.
-    2: { destruct step_fork eqn:SF; [| set_solver].
-         simpl. apply elem_of_disjoint.
-         intros ? [??]%elem_of_difference [->%elem_of_singleton ?]%elem_of_difference.
-         apply step_fork_difference in SF. set_solver. }
-    iFrame "PHS".
-
-    iSplitL "PH'".
-    { destruct step_fork eqn:SF.
-      2: { simpl. rewrite subseteq_empty_difference_L; set_solver. }
-      simpl. rewrite difference_disjoint_L.
-      { by rewrite big_sepS_singleton. }
-      apply elem_of_disjoint. intros ? ?%elem_of_singleton ?%elem_of_singleton. 
-      subst.
-      apply step_fork_difference in SF.
-      apply locales_of_cfg_step in STEP. set_solver. }
-    iFrame. done. 
-  Qed.
-
-  Lemma cur_obls_sigs_other_step `{!ObligationsGS Σ}
-    etr c' τ
-    (STEP: locale_step (trace_last etr) (Some τ) c')
-    (OTHER: τ ≠ τi)
-    :
-    cur_obls_sigs etr -∗
-      obls τ ∅ ∗ obls_τi' (trace_last etr) ∗
-      let oτ' := step_fork (trace_last etr) c' in
-      (obls τ ∅ -∗ obls_τi' c' -∗ (∀ τ', ⌜ oτ' = Some τ' /\ τ' ≠ τi ⌝ → obls τ' ∅) -∗
-       cur_obls_sigs (etr :tr[ Some τi ]: c')).
-  Proof using.
-    simpl. iIntros "(OBLS & OBτi)". iFrame "OBτi". 
-    rewrite /cur_obls_sigs. simpl.
-    iDestruct (big_sepS_elem_of_acc with "[$]") as "(OB & OBLS)".
-    { apply elem_of_difference. split; [| apply not_elem_of_singleton]; eauto.
-      eapply locales_of_cfg_step; eauto. }
-    iFrame "OB". iIntros "OB OBτi OB'".
-    iSpecialize ("OBLS" with "[$]").     
-    pose proof STEP as ->%locale_step_step_fork_exact.    
-    rewrite difference_union_distr_l_L big_sepS_union.
-    2: { destruct step_fork eqn:SF; [| set_solver].
-         simpl. apply elem_of_disjoint.
-         intros ? [??]%elem_of_difference [->%elem_of_singleton ?]%elem_of_difference.
-         apply step_fork_difference in SF. set_solver. }
-    iFrame.
-    destruct step_fork eqn:SF; simpl. 
-    2: { rewrite subseteq_empty_difference_L; set_solver. }
-    destruct (decide (l = τi)).
-    { rewrite subseteq_empty_difference_L; set_solver. } 
-    rewrite difference_disjoint_L; [| set_solver].
-    rewrite big_sepS_singleton. by iApply "OB'". 
-  Qed.
-
-  (* TODO: refactor *)
-  Lemma cur_phases_other_step `{!ObligationsGS Σ} etr c' τ
-    (STEP: locale_step (trace_last etr) (Some τ) c')
-    (* (etr' := etr :tr[ Some τi ]: c') *)
-    (etr' := etr :tr[ Some τ ]: c')
-    (FITS: fits_inf_call ic m ai etr')
-    (OTHER: τ ≠ τi):
-    cur_phases etr -∗
-    let oτ' := step_fork (trace_last etr) c' in
-    let ph := ∃ π, th_phase_eq τ π in
-    ph ∗ (ph -∗ from_option (fun τ' => ∃ π', th_phase_eq τ' π') ⌜ True ⌝ oτ' -∗
-          cur_phases etr' ∗
-          (⌜ trace_length etr = ii ⌝ → ∃ π, th_phase_frag τi π (/2)%Qp)).
-  Proof using.
-    clear WFST F.
-    rewrite /cur_phases. simpl. iIntros "(PHS & PHτi)".
-    iDestruct (big_sepS_elem_of_acc with "[$]") as "(PH & PHS)".
-    { apply elem_of_difference. split; [| apply not_elem_of_singleton]; eauto.
-      eapply locales_of_cfg_step; eauto. }
-    iFrame "PH". iIntros "PH PH'".
-    iSpecialize ("PHS" with "[$]"). 
-    pose proof STEP as ->%locale_step_step_fork_exact. 
-    rewrite difference_union_distr_l_L big_sepS_union.
-    2: { destruct step_fork eqn:SF; [| set_solver].
-         simpl. apply elem_of_disjoint.
-         intros ? [??]%elem_of_difference [->%elem_of_singleton ?]%elem_of_difference.
-         apply step_fork_difference in SF. set_solver. }
-    iFrame "PHS". rewrite -bi.sep_assoc. 
-    
-    destruct step_fork eqn:SF.
-    2: { simpl. iSplitR.
-         { rewrite subseteq_empty_difference_L; [| done]. set_solver. }
-         rewrite union_empty_r_L. 
-         destruct (decide (trace_length etr = ii)).
-         - destruct FITS. 
-           rewrite trace_lookup_last in fic_call .
-           2: { simpl in *. lia. }
-           simpl in fic_call. 
-           iSpecialize ("PHτi" with "[]").
-           { iPureIntro. red in fic_call. 
-             pose proof STEP as EQ%locale_step_step_fork_exact.
-             rewrite SF /= union_empty_r_L in EQ. rewrite -EQ.
-             eapply expr_at_in_locales; eauto. }
-           iDestruct "PHτi" as (?) "PH".
-           rewrite leb_correct; [| simpl in *; lia].
-           iDestruct (th_phase_frag_halve with "PH") as "[PH PH_]".
-           rewrite leb_correct_conv; [| simpl in *; lia].
-           rewrite half_inv2. iSplitL "PH".
-           + iIntros "_". iFrame.
-           + iIntros "_". iFrame.
-         - iSplitL.
-           2: { by iIntros (?). }
-           simpl. 
-           assert (S (trace_length etr) <=? ii = (trace_length etr <=? ii)) as X. 
-           2: { rewrite X. iFrame. }
-           simpl in *.
-           destruct (decide (trace_length etr <= ii)) as [LE | GT]. 
-           + by do 2 (rewrite leb_correct; [| lia]).
-           + by do 2 (rewrite leb_correct_conv; [| lia]). }
-
-    simpl. 
-    destruct (decide (l = τi)) as [-> | ?]. 
-    { rewrite subseteq_empty_difference_L; [| set_solver]. iSplitR; [set_solver| ].
-      iDestruct "PH'" as (?) "PH".
-      destruct (decide (trace_length etr = ii)).
-      - rewrite leb_correct; [| simpl in *; lia].
-        iDestruct (th_phase_frag_halve with "PH") as "[PH PH_]".
-        rewrite leb_correct_conv; [| simpl in *; lia].
-        rewrite half_inv2. iSplitL "PH".
-        + iIntros "_". iFrame.
-        + iIntros "_". iFrame.
-      - iSplitL.
-        2: { by iIntros (?). }
-        simpl.
-        iClear "PHτi". iIntros "_".
-        rewrite leb_correct; [iFrame| ].
-        enough ((trace_length etr) ≤ ii).
-        { simpl in *. lia. }
-        destruct (Nat.le_gt_cases (trace_length etr) ii); [done| ].
-        eapply fic_has_τi in H. 
-        2: { eapply fits_inf_call_prev; eauto. }
-        apply step_fork_difference in SF. set_solver. }
-
-    simpl. rewrite difference_disjoint_L.
-    2: { set_solver. }
-    rewrite big_opS_singleton. iFrame "PH'".
-
-    destruct (decide (trace_length etr = ii)).
-    - destruct FITS. subst etr'.
-      rewrite trace_lookup_last in fic_call.
-      2: { simpl in *. lia. }
-      simpl in fic_call.
-      iSpecialize ("PHτi" with "[]").
-      { iPureIntro. red in fic_call. 
-        pose proof STEP as EQ%locale_step_step_fork_exact.
-        rewrite SF /= in EQ.
-        apply expr_at_in_locales in fic_call. rewrite EQ in fic_call.
-        apply elem_of_union in fic_call as [|]; eauto.
-        set_solver. }
-      iDestruct "PHτi" as (?) "PH".
-      rewrite leb_correct; [| simpl in *; lia].
-      iDestruct (th_phase_frag_halve with "PH") as "[PH PH_]".
-      rewrite leb_correct_conv; [| simpl in *; lia].
-      rewrite half_inv2. iSplitL "PH".
-      + iIntros "_". iFrame.
-      + iIntros "_". iFrame.
-    - iSplitL. 
-      2: { by iIntros (?). }
-      simpl. 
-      assert (S (trace_length etr) <=? ii = (trace_length etr <=? ii)) as X. 
-      2: { rewrite X.
-           iIntros (?). iApply "PHτi".
-           iPureIntro. set_solver. }
-      simpl in *.
-      destruct (decide (trace_length etr <= ii)) as [LE | GT]. 
-      + by do 2 (rewrite leb_correct; [| lia]).
-      + by do 2 (rewrite leb_correct_conv; [| lia]).
-  Qed.
-
-  Lemma obls_τi'_next `{!ObligationsGS Σ} c c'
-    (SAME: locales_of_cfg c' = locales_of_cfg c):
-    obls_τi' c ⊣⊢ obls_τi' c'.
-  Proof using.
-    rewrite /obls_τi'. by rewrite SAME.
-  Qed.
-
-  Lemma BOU_wait_τi `{!ObligationsGS Σ} `{invGS_gen HasNoLc Σ} τ π:
-    obls τ ∅ -∗ th_phase_eq τ π -∗ obls_τi -∗
-      BOU ∅ WF_SB (cp π d0 ∗ th_phase_eq τ π ∗ obls τ ∅ ∗ obls_τi). 
-  Proof using.
-    clear m WFST F. 
-    iIntros "OB PH OBτi".
-    rewrite /obls_τi. iDestruct "OBτi" as "(%s & OBτi & SGN & #EP)".    
-    iMod (expect_sig_upd with "[] [$] OB [] [$]") as "(?&?&?&?)".
-    { iApply (ep_weaken with "[$]"). apply (phase_le_init π). } 
-    { (* TODO: Make a lemma *)
-      rewrite /sgns_level_gt. rewrite /sgns_levels_gt'.
-      iApply empty_sgns_levels_rel. }
-    { rewrite /WF_SB. lia. }
-    iModIntro. iFrame "#∗".
   Qed.
 
   Lemma wptp_wfree_other_simpl {Σ} {PWT: PrWfreeTok Σ}
@@ -876,110 +362,6 @@ Section WaitFreePR.
     (* (FIT: fits_inf_call ic m ai (etr :tr[ oτ ]: c')) *)
   .
 
-  Lemma locale_tp_split
-    (e e' : expr) (σ' : state) (efs t1 t2 : list expr)
-    (Heqc': (t1 ++ e' :: t2 ++ efs, σ') = c')
-    (τ := locale_of t1 e):
-    (locale_of t1 e ∉ locales_of_list t1) ∧
-    (locale_of t1 e ∉ locales_of_list_from (t1 ++ [e']) t2) ∧
-    locale_of t1 e ∉ locales_of_list_from (t1 ++ [e'] ++ t2) efs.
-  Proof using.
-    clear FIN VALID. 
-    pose proof (thread_pool_split c'.1 τ) as SPLIT.
-    rewrite -Heqc' /= in SPLIT. destruct SPLIT as (tp1 & tp2 & tp' & EQ & TP' & NO1 & NO2).
-    destruct TP' as [-> | (e_ & -> & LOC)].
-    { simpl in EQ.
-      assert (τ ∈ locales_of_list c'.1) as IN. 
-      { rewrite -Heqc' /=.
-        rewrite locales_of_list_from_app /=. rewrite locales_of_list_from_cons.
-        set_solver. }
-      rewrite -Heqc' /= EQ in IN.
-      rewrite locales_of_list_from_app /= in IN.
-      rewrite app_nil_r in NO2.
-      exfalso. 
-      apply elem_of_app in IN as [?|?]; eauto. }
-    rewrite -/τ /locale_of in LOC.
-    apply app_inj_1 in EQ as [EQ1 EQ2]; eauto.
-    simpl in EQ2. inversion EQ2. subst.
-    split; eauto.
-    apply Decidable.not_or. intros IN. destruct NO2.
-    rewrite locales_of_list_from_app. apply elem_of_app.
-    by rewrite -app_assoc.
-  Qed.
-
-  (* Lemma get_MU_impl *)
-  (* (e : expr) *)
-  (* (σ : state) *)
-  (* (e' : expr) *)
-  (* (σ' : state) *)
-  (* (efs t1 t2 : list expr) *)
-  (* (FIN : trace_last etr = (t1 ++ e :: t2, σ)) *)
-  (* (H : (t1 ++ e :: t2, σ) = c) *)
-  (* (τ : nat) *)
-  (* (H1 : (t1 ++ e' :: t2 ++ efs, σ') = c') *)
-  (* (STEP : locale_step (t1 ++ e :: t2, σ) (Some τ) (t1 ++ e' :: t2 ++ efs, σ')) *)
-  (* (π : Phase) *)
-  (* (sf : olocale heap_lang) *)
-  (* (Heqsf : sf = step_fork (trace_last etr) (t1 ++ e' :: t2 ++ efs, σ')) *)
-  (* (upd := fun (R1 R2: gset SignalId) => let _: ObligationsGS Σ := @iem_fairnessGS _ _ _ _ _ Hinv in *)
-  (*                       (⌜ R1 = ∅ ⌝ ∗  *)
-  (*                       if (decide (sf = Some τi)) *)
-  (*                       then (∃ s, ⌜ R2 = {[ s ]} ⌝ ∗ sgn s l0 (Some false) ∗ ep s π0 d0)%I *)
-  (*                       else (⌜ R2 = ∅ ⌝ ∗ obls_τi' (t1 ++ e' :: t2 ++ efs, σ')))%I) *)
-  (* (* "INV" : wfree_trace_inv etr mtr *) *)
-  (* (* cp π0 d0 -∗ th_phase_eq τ π -∗ obls τ ∅ -∗ obls_τi' (trace_last etr) -∗  *) *)
-
-  (* : *)
-  
-  (* ⊢ *)
-  (*   (* MU_impl *) *)
-  (*   let hGS: @heapGS Σ M EM := {| heap_iemgs := Hinv |} in *)
-  (*   @MU_impl _ EM Σ hGS sf ⊤ τ *)
-  (*   (∃ R1 R2 : gset SignalId, cp π0 d0 ∗ th_phase_eq τ π0 ∗  *)
-  (*      obls τ (R1 ∪ R2) ∗ upd R1 R2 ∗ ⌜R1 ## R2⌝).  *)
-  (* Proof using. *)
-  (*   iIntros "CP PH OB OBτi". *)
-
-  Lemma τi_not_in e σ e' σ'
-  (efs t1 t2 : list expr)
-  (FIN' : trace_last etr = (t1 ++ e :: t2, σ))
-  (τ := locale_of t1 e : nat)
-  (STEP : locale_step (t1 ++ e :: t2, σ) (Some τ) (t1 ++ e' :: t2 ++ efs, σ'))
-  (NO : step_fork (trace_last etr) (t1 ++ e' :: t2 ++ efs, σ') ≠ Some τi)
-  (FIT : from_locale (t1 ++ e' :: t2 ++ efs) τi = Some (fill Ki (m ai)))
-  (sf := step_fork (trace_last etr) (t1 ++ e' :: t2 ++ efs, σ')):
-  τi ∉ locales_of_list_from (t1 ++ e' :: t2) efs.
-  Proof using.
-    clear WFST F. 
-    rewrite locales_of_list_from_locales.
-    intros [[??] IN]%elem_of_list_In%in_map_iff.
-    destruct IN as (LOC & IN).
-    apply elem_of_list_In, elem_of_list_lookup in IN as [i IN].
-    pose proof IN as X.
-    apply prefixes_from_ith_length in IN. 
-    rewrite !length_app /= in IN. rewrite /locale_of in LOC.
-    
-    apply from_locale_lookup in FIT.
-    apply lookup_lt_Some in FIT. simpl in FIT.
-    rewrite /τi in LOC.
-    rewrite /τi -LOC IN in FIT. 
-    repeat rewrite !length_app /= in FIT.
-    simpl in FIT.
-    
-    apply step_fork_hl in STEP as [[? ->] | (?&->&?)].
-    { simpl. simpl in FIT. lia. }
-    simpl in FIT. destruct i; [| lia].
-    simpl in X. inversion X.
-    subst. simpl in e0.
-    rewrite app_comm_cons app_assoc in NO.
-    rewrite FIN' in NO.
-    rewrite step_fork_fork in NO.
-    { rewrite /τi in NO. 
-      rewrite -LOC in NO. 
-      rewrite /locale_of !length_app in NO. done. }
-    apply locales_equiv_middle. done.
-  Qed.    
-
   Lemma unfold_helper (STEP: locale_step c oτ c'):
     wptp_wfree s etr Φs -∗
     ∃ e t1 t2 efs e' Φs1 Φ Φs2,
@@ -1027,17 +409,6 @@ Section WaitFreePR.
     by subst.
   Qed.
     
-  (* (* H3: *) *)
-  (* H3 : locale_of t1 e = τ *)
-  (* H : (t1 ++ e :: t2, σ) = c *)
-  (* H1 : (t1 ++ e' :: t2 ++ efs, σ') = c' *)
-  (* EQ :  Φs1 ++ Φs' = Φs /\ *)
-  (* LEN1 : length Φs1 = length t1 *)
-  (* LEN' : length Φs' = length (e :: t2) *)
-  (* Φ : val → iPropI Σ *)
-  (* Φs2 : list (val → iPropI Σ) *)
-  (* EQ' : [Φ] ++ Φs2 = Φs' *)
-
   Lemma no_ongoing_call
     (e': expr) (K : ectx heap_lang) (s0 : nat) τ c''
     (FIT : fits_inf_call ic m ai (etr :tr[ τ ]: c''))
@@ -1084,6 +455,8 @@ Section WaitFreePR.
     eapply Forall2_app; [apply adequacy_utils.locales_equiv_refl| ].
     simpl. by constructor.
   Qed.
+
+  #[local] Arguments Nat.leb _ _ : simpl nomatch.
 
   Lemma wptp_wfree_take_step_τi
     (EQ_TID: oτ = Some τi)
@@ -1227,8 +600,8 @@ Section WaitFreePR.
         rewrite leb_correct; [| simpl in *; lia].
         iSpecialize ("PHS" with "[PH]"); [by eauto| ].
                     
-        iAssert (cur_phases (etr :tr[ Some (locale_of t1 e) ]: (t1 ++ e' :: t2 ++ efs, σ')) ∗
-                   cur_obls_sigs (etr :tr[ Some (locale_of t1 e) ]: (t1 ++ e' :: t2 ++ efs, σ')))%I with "[-CTI]" as "[PHS OBS]".
+        iAssert (cur_phases ic (etr :tr[ Some (locale_of t1 e) ]: (t1 ++ e' :: t2 ++ efs, σ')) ∗
+                   cur_obls_sigs ic (etr :tr[ Some (locale_of t1 e) ]: (t1 ++ e' :: t2 ++ efs, σ')))%I with "[-CTI]" as "[PHS OBS]".
         { destruct step_fork eqn:SF; simpl. 
           - iDestruct "MOD'" as (?) "(PH' & OB & OB')".
             iSplitL "PH' PHS".
@@ -1267,14 +640,14 @@ Section WaitFreePR.
 
         iFrame "WPS".
         iSpecialize ("CPS" with "[]").
-        { iIntros (?). simpl in H0. lia. }
+        { iIntros (?). simpl in *. lia. }
         iFrame "CPS".
         rewrite leb_correct_conv; [| simpl in *; lia].
         iSpecialize ("PHS" with "[PH]").
         { rewrite half_inv2. iFrame. }
 
-        iAssert (cur_phases (etr :tr[ Some (locale_of t1 e) ]: (t1 ++ e' :: t2 ++ efs, σ')) ∗
-                   cur_obls_sigs (etr :tr[ Some (locale_of t1 e) ]: (t1 ++ e' :: t2 ++ efs, σ')))%I with "[-]" as "[PHS OBS]".
+        iAssert (cur_phases ic (etr :tr[ Some (locale_of t1 e) ]: (t1 ++ e' :: t2 ++ efs, σ')) ∗
+                   cur_obls_sigs ic (etr :tr[ Some (locale_of t1 e) ]: (t1 ++ e' :: t2 ++ efs, σ')))%I with "[-]" as "[PHS OBS]".
         { destruct step_fork eqn:SF; simpl. 
           - iDestruct "MOD'" as (?) "(PH' & OB & OB')".
             iSplitL "PH' PHS".
@@ -1396,98 +769,6 @@ Section WaitFreePR.
     by iApply (bump_cti with "[$]"). 
   Qed.
 
-  (* TODO: this doesn't rely on (oτ ≠ Some τi)? can it be reused?*)
-  Lemma take_model_step t1 e' t2 efs σ' π e
-    (oτ' := step_fork c (t1 ++ ectx_fill ectx_emp e' :: t2 ++ efs, σ'))
-    (τ := locale_of t1 e)
-    (FIN': trace_ends_in etr c)
-    (STEP: locale_step c (Some τ) (t1 ++ ectx_fill ectx_emp e' :: t2 ++ efs, σ'))
-:
-    let oGS: ObligationsGS Σ := @iem_fairnessGS _ _ _ _ _ (@pwt_Hinv _ PWT) in
-    cp π0 d0 -∗ th_phase_eq τ π -∗ obls (locale_of t1 e) ∅ -∗ obls_τi' (trace_last etr) -∗     
-    @MU_impl _
-          EM Σ {| heap_iemgs := @pwt_Hinv Σ PWT |} oτ' ⊤
-          τ
-          (∃ (π0 : Phase) (R1 R2 : @gset SignalId Nat.eq_dec nat_countable),
-             @th_phase_eq Degree Level (locale heap_lang) WF_SB OP Σ
-               _
-               τ π0 ∗
-             (λ R0 R3 : @gset SignalId Nat.eq_dec nat_countable,
-                let H :=
-                  @iem_fairnessGS heap_lang
-                    (AM2M
-                       (@ObligationsAM Degree Level (locale heap_lang) WF_SB OP
-                          Nat.inhabited))
-                    HeapLangEM EM Σ Hinv
-                  in
-                ⌜R0 = ∅⌝ ∗
-                (if
-                  decide (oτ' = @Some (locale heap_lang) τi)                    
-                 then
-                  ∃ s0, ⌜R3 = {[s0]}⌝ ∗
-                    @sgn Degree unitO (locale heap_lang) WF_SB OP Σ H s0 l0
-                      (@Some bool false) ∗
-                    @ep (@sigO natO (λ i : nat, i < 2)) Level
-                      (locale heap_lang) WF_SB OP Σ H s0 obligations_model.π0 d0
-                 else ⌜R3 = ∅⌝ ∗ @obls_τi' Σ H (t1 ++ e' :: t2 ++ efs, σ')))
-               R1 R2 ∗
-             ⌜R1 ## R2⌝ ∗
-             @from_option (locale heap_lang) (iPropI Σ)
-               (λ τ' : locale heap_lang,
-                  ∃ π' : Phase,
-                    @th_phase_eq Degree Level (locale heap_lang) WF_SB OP Σ
-                      _
-                      τ' π' ∗
-                    @obls Degree Level (locale heap_lang) WF_SB OP Σ _ τ R1 ∗
-                    @obls Degree Level (locale heap_lang) WF_SB OP Σ _ τ' R2)
-               (@obls Degree Level (locale heap_lang) WF_SB OP Σ _ τ (R1 ∪ R2))
-               oτ').
-  Proof using.
-    clear m WFST VALID FIN F. 
-    simpl. iIntros "CP PH OB OBτi".
-    rewrite (cp_weaken _ π); [| by apply phase_le_init].
-    rewrite /obls_τi' /obls_τi.
-    
-    iApply (MU_burn_cp with "[-]").
-    iFrame "CP PH". simpl.
-    rewrite -FIN' in STEP.
-
-    assert (exists sf, sf = oτ') as (sf & Heqsf) by eauto. subst oτ'.
-    rewrite FIN' in STEP.
-    rewrite -Heqsf. 
-
-    destruct sf; simpl.
-    2: { iModIntro. do 2 iExists _.
-         iSplitL "OB".
-         { erewrite union_empty_r_L. iFrame. }
-         repeat (iSplit; try done).
-         iApply obls_τi'_next; [| done].
-         apply locale_step_step_fork_exact in STEP.
-         rewrite -Heqsf /= in STEP.
-         rewrite STEP. rewrite FIN'. set_solver. }
-    destruct (decide (l = τi)) as [-> | NEQ].
-    - rewrite decide_False.
-      2: { eapply locale_step_fork_Some in STEP; eauto.
-           rewrite FIN'. tauto. }
-      iMod (OU_create_sig with "[$]") as "(%sg & SGN & OB & _)".
-      { rewrite /WF_SB. lia. }
-      iDestruct (sgn_get_ex with "[$]") as "(SGN & #SGN0)".
-      iMod (create_ep_upd with "[OBτi] SGN0") as "(#EP & _)".
-      { apply (orders_lib.ith_bn_lt 2 0 1). lia. }
-      { iFrame. }
-      iModIntro. do 2 iExists _. rewrite decide_True; [| done].
-      iFrame. iFrame "#∗". iPureIntro. set_solver.
-    - iModIntro. iFrame.
-      setoid_rewrite (@decide_False _ (Some l = _)); [| congruence].
-      do 2 iExists _. erewrite union_empty_r_L. iFrame.
-      repeat iSplit; try done.
-      rewrite /obls_τi'.
-      apply locale_step_step_fork_exact in STEP. rewrite STEP.
-      erewrite decide_ext; [by iFrame| ].
-      rewrite -Heqsf. simpl.
-      rewrite FIN'. set_solver.
-  Qed.
-
   Lemma wptp_wfree_take_step'_other
     (STEP: locale_step c oτ c')
     (OTHER: oτ ≠ Some τi)
@@ -1522,11 +803,11 @@ Section WaitFreePR.
       iDestruct (split_trace_fuel with "[$]") as "(CP & CPP & CPS)"; [done| ].
       iDestruct (cur_obls_sigs_other_step with "[$]") as "(OB & OBτi & OBLS)".
       { by rewrite FIN. }
-      { congruence. }
-      iDestruct (cur_phases_other_step _ _ τ with "[$]") as "(PH & PHS)".
+      { set_solver. }
+      iDestruct (cur_phases_other_step _ _ _ τ with "[$]") as "(PH & PHS)".
       { rewrite FIN. subst τ. eauto. }
       { eauto. }
-      { subst τ. congruence. }
+      { subst τ. set_solver. }
       iDestruct "PH" as (π) "PH". 
 
       remember (step_fork (trace_last etr) (t1 ++ e' :: t2 ++ efs, σ')) as sf.
@@ -1537,7 +818,7 @@ Section WaitFreePR.
       { done. }
       { done. }
       { iPoseProof (take_model_step with "[$] [$] [$] [$]") as "foo".
-        { congruence. }
+        { set_solver. }
         { rewrite ectx_fill_emp. subst c. eauto. }
         rewrite ectx_fill_emp.
         rewrite FIN. subst τ c.  
@@ -1736,13 +1017,13 @@ Section WaitFreePR.
     + apply leb_complete_conv in LEN. simpl in LEN.
 
       iClear "CPS".
-      iAssert (extra_fuel (etr :tr[ Some τ ]: (t1 ++ e' :: t2 ++ efs, σ'))) as "CPS'".
+      iAssert (extra_fuel ic F (etr :tr[ Some τ ]: (t1 ++ e' :: t2 ++ efs, σ'))) as "CPS'".
       { rewrite /extra_fuel. rewrite leb_correct_conv; [done| ].
         simpl. lia. }
         
       iDestruct (cur_obls_sigs_other_step with "[$]") as "(OB & OBτi & OBLS)".
       { by rewrite FIN. }
-      { congruence. }
+      { set_solver. }
       iDestruct (cur_phases_other_step with "[$]") as "(PH & PHS)"; eauto.
       { rewrite FIN. subst τ. eauto. }
       iDestruct "PH" as (π) "PH". 
@@ -1759,7 +1040,7 @@ Section WaitFreePR.
       { done. }
       { done. }
       { rewrite -Heqsf. 
-        iApply (MU_burn_cp _ _ _ _ (fun (R1 R2: gset SignalId) => (⌜ R1 = ∅ /\ R2 = ∅⌝ ∗ obls_τi)%I) with "[-]").
+        iApply (MU_burn_cp _ _ _ _ (fun (R1 R2: gset SignalId) => (⌜ R1 = ∅ /\ R2 = ∅⌝ ∗ (obls_τi ic))%I) with "[-]").
         iMod (BOU_wait_τi with "[$] [$] [$]") as "(?&?&OB&?)".
         iModIntro. do 2 iExists _. iFrame.  
         iSplitL "OB".
